reflection/tactics: distinguish Tv_Unknown and Tv_Unsupp

src/reflection/FStar.Reflection.Data.fsti
@@ -100,6 +100,7 @@ type term_view =
                                                          //see also Syntax
     | Tv_AscribedC of term * comp * option term * bool  //bool is similar to Tv_AscribedT
     | Tv_Unknown
+    | Tv_Unsupp
 
 val notAscription (t:term_view) : Tot bool
 
